We measure $p_\mu^\mu$ and $\vec{p}_T^\nu$. 

We will impose ${p_\mu^{\rm{comb.}}}^2 = m_W^2$

Assume $p_\nu^2 = p_\mu^2 = 0$. Only unknown is $p_z^\nu$


$p_\mu^{\rm{comb.}} = \begin{pmatrix} E_\mu + E_\nu \\  \vec{p}_T^\mu + \vec{p}_T^\nu \\ {p_z}_\mu + {p_z}_\nu \end{pmatrix}$ 


${p_\mu^{\rm{comb.}}}^2 = (E_\mu + E_\nu)^2 - \left[ (\vec{p}_T^\mu + \vec{p}_T^\nu)^2 + ({p_z}_\mu + {p_z}_\nu)^2 \right]$

$= \cancel{|p_\mu|^2} + 2|p_\mu| |p_\nu| + \cancel{|p_\nu|^2} - \left[ \cancel{{\vec{p}_T^\mu}^2} + {\cancel{\vec{p}_T^\nu}^2} + 2 \vec{p}_T^\mu \cdot \vec{p}_T^\nu  + \cancel{{{p_z}_\mu}^2} + \cancel{{{p_z}_\nu}^2} + 2{p_z}_\mu{p_z}_\nu   \right]$

OR

$m_W^2 = 2 E_\mu \sqrt{ {\vec{p}_T^\nu}^2 + {{p_{z}}_\nu}^2 } - 2 \left[ \vec{p}_T^\mu \cdot \vec{p}_T^\nu + {p_z}_\mu {p_z}_\nu \right]$

$\frac{m_W^2}{2} + \left[ \vec{p}_T^\mu \cdot \vec{p}_T^\nu + {p_z}_\mu {p_z}_\nu \right] = E_\mu \sqrt{ {\vec{p}_T^\nu}^2 + {{p_{z}}_\nu}^2 }$

Squaring

$\frac{m_W^4}{4} + m_W^2 \left[ \vec{p}_T^\mu \cdot \vec{p}_T^\nu + {p_z}_\mu {p_z}_\nu \right] + \left[ \vec{p}_T^\mu \cdot \vec{p}_T^\nu + {p_z}_\mu {p_z}_\nu \right]^2 = E_\mu^2 ( {\vec{p}_T^\nu}^2 + {{p_{z}}_\nu}^2 )$

$\frac{m_W^4}{4} + m_W^2 \left[ \vec{p}_T^\mu \cdot \vec{p}_T^\nu + {p_z}_\mu {p_z}_\nu \right] + \left[ (\vec{p}_T^\mu \cdot \vec{p}_T^\nu)^2 + 2(\vec{p}_T^\mu \cdot \vec{p}_T^\nu) {p_z}_\mu {p_z}_\nu + ({p_z}_\mu {p_z}_\nu)^2 \right] = E_\mu^2 ( {\vec{p}_T^\nu}^2 + {{p_{z}}_\nu}^2 )$

OR ...

$\left( \frac{m_W^4}{4} + m_W^2 \vec{p}_T^\mu \cdot \vec{p}_T^\nu  + (\vec{p}_T^\mu \cdot \vec{p}_T^\nu)^2 -  E_\mu^2 {\vec{p}_T^\nu}^2  \right) + \left(m_W^2{p_z}_\mu + 2(\vec{p}_T^\mu \cdot \vec{p}_T^\nu){p_z}_\mu \right){p_z}_\nu +  \left( {p_z}_\mu^2 - E_\mu^2 \right){{p_z}_\nu}^2 =0$

which is 

$C + B \cdot {p_z}_\nu + A \cdot {{p_z}_\nu}^2 = 0$

with

$A = \left( {p_z}_\mu^2 - E_\mu^2 \right)$

$B = \left(m_W^2{p_z}_\mu + 2(\vec{p}_T^\mu \cdot \vec{p}_T^\nu){p_z}_\mu \right)$

$C = \left( \frac{m_W^4}{4} + m_W^2 \vec{p}_T^\mu \cdot \vec{p}_T^\nu  + (\vec{p}_T^\mu \cdot \vec{p}_T^\nu)^2 -  E_\mu^2 {\vec{p}_T^\nu}^2  \right)$

Then have two solutions for ${p_z}_\nu$.

${p_z}_\nu = \frac{-B \pm \sqrt{B^2 - 4AC}}{2A}$



## Follow-ups


## Links: 
[[Physics]]



202410031242
