Claim
$$
\Delta R \sim \frac{2m}{p_T}
$$

Proof:
$$
	E^2 = p^2 + m^2
$$
$$
m^2 = (E_1^2 + E_2^2)^2 - (\vec{p}_1^2 + \vec{p}_1^2 )^2
$$
Assume particles 1 and 2 are massless:
$$     = (p_1^2 + p_2^2 + 2 p_1 p_2) - (|p_1|^2 + |p_2|^2 + 2|p_1||p_2|\cos(\Delta\phi)) $$
$$     = 2|p_1||p_2|(1- \cos(\Delta\phi) $$
$$     = 2|p_1||p_2|(1- (1 - (\frac{\Delta R}{2})^2) $$
$$     = |p_1||p_2|(\Delta R)^2 $$

Assume $$ |p_1| \sim |p_2| \sim p_C/2$$
Then 
$$\Delta R^2 \sim \frac{4 m^2}{p_T^2}  $$
or
$$\Delta R \sim \frac{2 m}{p_T}  $$
## Follow-ups


## Links: 
[[Physics]]


202408021713
